[
  {
    "@id": "https://valospace.org/index",
    "@context": {
      "@base": "https://valospace.org/index#",
      "sbomdoc": "https://valospace.org/sbomdoc#",
      "revdoc": "https://valospace.org/revdoc#",
      "rdf": "http://www.w3.org/1999/02/22-rdf-syntax-ns#",
      "rdfs": "http://www.w3.org/2000/01/rdf-schema#",
      "xsd": "http://www.w3.org/2001/XMLSchema#",
      "owl": "http://www.w3.org/2002/07/owl#",
      "dc": "http://purl.org/dc/elements/1.1/",
      "vdoc": "https://valospace.org/vdoc#",
      "vdoc:content": {
        "@id": "https://valospace.org/vdoc#content",
        "@container": "@list",
        "@type": "@id"
      },
      "vdoc:words": {
        "@id": "https://valospace.org/vdoc#words",
        "@container": "@list",
        "@type": "@id"
      },
      "vdoc:entries": {
        "@id": "https://valospace.org/vdoc#entries",
        "@container": "@list",
        "@type": "@id"
      },
      "vdoc:headers": {
        "@id": "https://valospace.org/vdoc#headers",
        "@container": "@list",
        "@type": "@id"
      },
      "vdoc:cell": {
        "@id": "https://valospace.org/vdoc#cell",
        "@container": "@list",
        "@type": "@id"
      }
    },
    "dc:title": "Valospace reference",
    "vdoc:tags": [
      "PRIMARY",
      "INTRODUCTION",
      "ONTOLOGY",
      "VALONAUT"
    ],
    "revdoc:package": "@valos/kernel",
    "revdoc:prefix": "valos",
    "revdoc:prefixIRI": "https://valospace.org/#",
    "revdoc:version": "0.35.0-prerelease.11",
    "respecConfig": {
      "specStatus": "unofficial",
      "editors": [
        {
          "name": "Iridian Kiiskinen",
          "url": "https://valaatech.github.io/fabric/authors/iridian",
          "github": "http://github.com/valospace"
        }
      ],
      "authors": [],
      "shortName": "valos"
    },
    "documents": {
      "@id": "documents",
      "sbom": {
        "@id": "https://valospace.org/sbom",
        "tags": [
          "PRIMARY",
          "SBOM"
        ],
        "subProfiles": [],
        "title": "@valos/kernel@0.35.0-prerelease.10 Software Bill of Materials",
        "abstract": {
          "@type": "vdoc:Chapter",
          "vdoc:content": [
            "This document is an autogenerated",
            {
              "@type": "vdoc:Reference",
              "vdoc:content": [
                "CycloneDX"
              ],
              "vdoc:ref": "https://cyclonedx.org/"
            },
            {
              "@type": "vdoc:Reference",
              "vdoc:content": [
                "SBoM document"
              ],
              "vdoc:ref": "https://www.owasp.org/index.php/Component_Analysis#Software_Bill-of-Materials_.28SBOM.29"
            }
          ]
        },
        "introduction": {
          "@type": "vdoc:Chapter",
          "vdoc:content": [
            "Configure @valos/type-vault-sbom.introduction section using",
            {
              "@type": "vdoc:Reference",
              "vdoc:content": [
                "VDoc source graph syntax"
              ],
              "vdoc:ref": "@valos/vdoc#source_graph"
            },
            "to define the content of this section."
          ]
        },
        "package": "@valos/kernel",
        "version": "0.35.0-prerelease.10"
      },
      "engine": {
        "@id": "https://valospace.org/engine",
        "tags": [],
        "subProfiles": [],
        "title": "engine",
        "abstract": {
          "@type": "vdoc:Chapter",
          "vdoc:content": [
            "This document is a revdoc template document 'engine' created by write-revdoc."
          ]
        },
        "introduction": {
          "@type": "vdoc:Chapter",
          "vdoc:content": [
            "Edit me - this is the first payload chapter. Abstract and SOTD are essential",
            {
              "@type": "vdoc:Reference",
              "vdoc:content": [
                "ReSpec boilerplate"
              ],
              "vdoc:ref": "https://github.com/w3c/respec/wiki/ReSpec-Editor's-Guide#essential-w3c-boilerplate"
            },
            null,
            "See ",
            {
              "@type": "vdoc:Reference",
              "vdoc:content": [
                "ReVDoc tutorial"
              ],
              "vdoc:ref": "@valos/revdoc/tutorial"
            },
            " for instructions on how to write revdoc source documents.",
            null,
            "See also ",
            {
              "@type": "vdoc:Reference",
              "vdoc:content": [
                "ReVdoc specification"
              ],
              "vdoc:ref": "@valos/revdoc"
            },
            " and ",
            {
              "@type": "vdoc:Reference",
              "vdoc:content": [
                "VDoc specification"
              ],
              "vdoc:ref": "@valos/vdoc"
            },
            " for reference documentation."
          ]
        },
        "package": "@valos/engine",
        "version": "0.35.0-prerelease.10"
      },
      "inspire": {
        "@id": "https://valospace.org/inspire",
        "tags": [],
        "subProfiles": [],
        "title": "inspire",
        "abstract": {
          "@type": "vdoc:Chapter",
          "vdoc:content": [
            "This document is a revdoc template document 'inspire' created by write-revdoc."
          ]
        },
        "introduction": {
          "@type": "vdoc:Chapter",
          "vdoc:content": [
            "Edit me - this is the first payload chapter. Abstract and SOTD are essential",
            {
              "@type": "vdoc:Reference",
              "vdoc:content": [
                "ReSpec boilerplate"
              ],
              "vdoc:ref": "https://github.com/w3c/respec/wiki/ReSpec-Editor's-Guide#essential-w3c-boilerplate"
            },
            null,
            "See ",
            {
              "@type": "vdoc:Reference",
              "vdoc:content": [
                "ReVDoc tutorial"
              ],
              "vdoc:ref": "@valos/revdoc/tutorial"
            },
            " for instructions on how to write revdoc source documents.",
            null,
            "See also ",
            {
              "@type": "vdoc:Reference",
              "vdoc:content": [
                "ReVdoc specification"
              ],
              "vdoc:ref": "@valos/revdoc"
            },
            " and ",
            {
              "@type": "vdoc:Reference",
              "vdoc:content": [
                "VDoc specification"
              ],
              "vdoc:ref": "@valos/vdoc"
            },
            " for reference documentation."
          ]
        },
        "package": "@valos/inspire",
        "version": "0.35.0-prerelease.10"
      },
      "raem": {
        "@id": "https://valospace.org/raem",
        "tags": [
          "PRIMARY",
          "INTRODUCTORY",
          "ONTOLOGY",
          "LIBRARY"
        ],
        "subProfiles": [],
        "title": "ValOS Resources And Events Model (ValOS-RAEM) API, schema and ontology",
        "abstract": {
          "@type": "vdoc:Chapter",
          "vdoc:content": [
            "This library provides the definitions and reference implementation\nfor the fundamental ",
            {
              "@type": "vdoc:CharacterData",
              "vdoc:content": [
                "ValOS Resources"
              ]
            },
            " and ",
            {
              "@type": "vdoc:CharacterData",
              "vdoc:content": [
                "ValOS Events"
              ]
            },
            " systems."
          ]
        },
        "introduction": {
          "@type": "vdoc:Chapter",
          "vdoc:content": [
            "This library provides the definitions and reference implementations\nfor the fundamental ",
            {
              "@type": "vdoc:CharacterData",
              "vdoc:content": [
                "ValOS Resources"
              ]
            },
            " and ",
            {
              "@type": "vdoc:CharacterData",
              "vdoc:content": [
                "ValOS Events"
              ]
            },
            " systems.",
            null,
            "",
            {
              "vdoc:quote": true,
              "vdoc:content": [
                [
                  "A ValOS Resource ",
                  {
                    "@type": "vdoc:CharacterData",
                    "vdoc:content": [
                      "resource"
                    ]
                  },
                  " represents a well-defined part of\n  the world. It has a well-defined state at each particular moment in time."
                ]
              ]
            },
            "",
            null,
            "",
            {
              "vdoc:quote": true,
              "vdoc:content": [
                [
                  "A ValOS Event ",
                  {
                    "@type": "vdoc:CharacterData",
                    "vdoc:content": [
                      "event"
                    ]
                  },
                  " represents a dynamic change to a\n  resource by describing the change from previous to subsequent resource\n  states at a particular time."
                ]
              ]
            },
            "",
            null,
            "The interplay of these distinct yet interwoven systems forms the\nfoundation of the Valaa Open System."
          ]
        },
        "ontologyAbstract": {
          "vdoc:content": [
            "@valos/raem ontology specifies the Valospace core types and\n      properties directly to the @valos/kernel namespace. "
          ]
        },
        "package": "@valos/raem",
        "version": "0.35.0-prerelease.10"
      },
      "raem/valos-resource-id": {
        "@id": "https://valospace.org/raem/valos-resource-id",
        "tags": [],
        "subProfiles": [],
        "title": "ValOS Resource Identifier",
        "abstract": {
          "@type": "vdoc:Chapter",
          "vdoc:content": [
            "ValOS Resource Identifiers (*VRIDs*) uniquely identify valospace\nresources created and manipulated by ",
            {
              "@type": "vdoc:Reference",
              "vdoc:content": [
                "ValOS event logs"
              ],
              "vdoc:ref": "@valos/sourcerer/valos-event-log"
            },
            ".\nVRIDs are strings with restricted grammar so that they can be embedded\ninto various URI component and list formats without encoding.\n"
          ]
        },
        "introduction": {
          "@type": "vdoc:Chapter",
          "vdoc:content": [
            "A VRID is the NSS part of an urn:valos URI. It is a string with two\nnested levels of syntactic structure. The outer structure consists of\n`@`-separated segments.",
            null,
            "",
            {
              "@type": "revdoc:ABNF",
              "vdoc:language": "https://tools.ietf.org/html/rfc5234",
              "vdoc:content": [
                "\n  vrid           = vgrid-segment *( \"@\" sub-segment )\n"
              ]
            },
            "",
            null,
            "The vgrid-segment uniquely identifies a *global resource*. The\noptional sub-segments identify an unambiguous path from the\nglobal resource to a *structural sub-resource* which also is the\n*referenced resource* of the VRID. Otherwise if there are no\nsub-segments the global resource is the referenced resource.",
            null,
            "The inner structure consists of `$`-separated parts which specify\nthe semantics of each individual segment.",
            null,
            "",
            {
              "@type": "revdoc:ABNF",
              "vdoc:language": "https://tools.ietf.org/html/rfc5234",
              "vdoc:content": [
                "\n  vgrid-segment  = \"$\" vgrid-format-term \"$\" vgrid-body\n  sub-segment    = sub-type-term \"$\" sub-context-term \"$\" sub-body\n"
              ]
            },
            "",
            null,
            "The identified resource (and thus the VRID itself) is always affiliated\nwith an event log in the context where the VRID appears.\nThe *term* parts refer the event log JSON-LD context term definitions,\nboth for syntactic purposes (e.g. as simple prefix expansions) as well\nas semantically (JSON-LD constructs such as index maps have semantic\nmeaning for some VRID subsegments).",
            null,
            "The two *body* parts carry the actual encodeURIComponent-encoded\nsegment data. The precise meaning depends on the segment type (e.g. URI\nsuffix, member access etc.).\n"
          ]
        },
        "package": "@valos/raem",
        "version": "0.35.0-prerelease.10"
      },
      "revdoc": {
        "@id": "https://valospace.org/revdoc",
        "tags": [
          "PRIMARY",
          "ONTOLOGY"
        ],
        "subProfiles": [],
        "title": "ReVDoc - ReSpec document VDoc extension",
        "abstract": {
          "@type": "vdoc:Chapter",
          "vdoc:content": [
            "This document specifies ReVDoc, a ",
            {
              "@type": "vdoc:Reference",
              "vdoc:content": [
                "VDoc extension"
              ],
              "vdoc:ref": "@valos/vdoc#extension"
            },
            " for extracting and emitting ",
            {
              "@type": "vdoc:Reference",
              "vdoc:content": [
                "ReSpec documents"
              ],
              "vdoc:ref": "https://github.com/w3c/respec"
            },
            "."
          ]
        },
        "introduction": {
          "@type": "vdoc:Chapter",
          "vdoc:content": [
            "ReVDoc is a VDoc extension which can produce ReSpec documents."
          ]
        },
        "ontologyAbstract": {
          "vdoc:content": [
            "ReVDoc ontology provides vocabulary and definitions which are\n      tailored for emitting ReSpec html output documents."
          ]
        },
        "package": "@valos/revdoc",
        "version": "0.35.0-prerelease.10"
      },
      "revdoc/tutorial": {
        "@id": "https://valospace.org/revdoc/tutorial",
        "tags": [],
        "subProfiles": [],
        "title": "ReVDoc Tutorial",
        "abstract": {
          "@type": "vdoc:Chapter",
          "vdoc:content": [
            "This document is a revdoc template document 'tutorial' created by write-revdoc."
          ]
        },
        "introduction": {
          "@type": "vdoc:Chapter",
          "vdoc:content": [
            "Edit me - this is the first payload chapter. Abstract and SOTD are essential",
            {
              "@type": "vdoc:Reference",
              "vdoc:content": [
                "ReSpec boilerplate"
              ],
              "vdoc:ref": "https://github.com/w3c/respec/wiki/ReSpec-Editor's-Guide#essential-w3c-boilerplate"
            },
            null,
            "See ",
            {
              "@type": "vdoc:Reference",
              "vdoc:content": [
                "ReVDoc tutorial"
              ],
              "vdoc:ref": "@valos/revdoc/tutorial"
            },
            " for instructions on how to write revdoc source documents.",
            null,
            "See also ",
            {
              "@type": "vdoc:Reference",
              "vdoc:content": [
                "ReVdoc specification"
              ],
              "vdoc:ref": "@valos/revdoc"
            },
            " and ",
            {
              "@type": "vdoc:Reference",
              "vdoc:content": [
                "VDoc specification"
              ],
              "vdoc:ref": "@valos/vdoc"
            },
            " for reference documentation."
          ]
        },
        "package": "@valos/revdoc",
        "version": "0.35.0-prerelease.10"
      },
      "sbomdoc": {
        "@id": "https://valospace.org/sbomdoc",
        "tags": [
          "PRIMARY",
          "ONTOLOGY"
        ],
        "subProfiles": [],
        "title": "SBoMDoc - Software Bill of Materials VDoc extension",
        "abstract": {
          "@type": "vdoc:Chapter",
          "vdoc:content": [
            "This document specifies SBomDoc, a ",
            {
              "@type": "vdoc:Reference",
              "vdoc:content": [
                "VDoc extension"
              ],
              "vdoc:ref": "@valos/vdoc#extension"
            },
            " for extracting and emitting ",
            {
              "@type": "vdoc:Reference",
              "vdoc:content": [
                "CycloneDX BOM documents"
              ],
              "vdoc:ref": "https://cyclonedx.org/"
            },
            " in various formats."
          ]
        },
        "introduction": {
          "@type": "vdoc:Chapter",
          "vdoc:content": [
            "SBoMDoc is a VDoc extension which uses CycloneDX namespaces and\n    can emit BOM documents in various formats."
          ]
        },
        "ontologyAbstract": {
          "vdoc:content": [
            "SBoMDoc ontology provides vocabulary and definitions which are\n      tailored for representing CycloneDX SBoM analysis semantic\n      content."
          ]
        },
        "package": "@valos/sbomdoc",
        "version": "0.35.0-prerelease.10"
      },
      "script": {
        "@id": "https://valospace.org/script",
        "tags": [
          "PRIMARY",
          "INTRODUCTORY",
          "ONTOLOGY",
          "LIBRARY"
        ],
        "subProfiles": [],
        "title": "ValOS Script API, schema",
        "abstract": {
          "@type": "vdoc:Chapter",
          "vdoc:content": [
            "This library provides the definitions and reference implementation\n    for valoscript, the valospace ECMAScript dialect."
          ]
        },
        "introduction": {
          "@type": "vdoc:Chapter",
          "vdoc:content": [
            "Valoscript extends ECMAScript 5 object model transparently for\nmanipulating valospace resources. The valoscript interpreter creates ",
            {
              "@type": "vdoc:Reference",
              "vdoc:content": [
                "events"
              ],
              "vdoc:ref": "@valos/raem#event"
            },
            " from all valospace resource\nmodification side-effects and groups all such side effects into\ntransactions. Valoscript retains ECMAScript 5 syntax and semantics."
          ]
        },
        "ontologyAbstract": {
          "vdoc:content": [
            "@valos/script ontology specifies the Valospace core types and\n      properties directly to the @valos/kernel namespace. "
          ]
        },
        "package": "@valos/script",
        "version": "0.35.0-prerelease.10"
      },
      "sourcerer": {
        "@id": "https://valospace.org/sourcerer",
        "tags": [
          "PRIMARY",
          "INTRODUCTORY",
          "ONTOLOGY",
          "LIBRARY"
        ],
        "subProfiles": [],
        "title": "ValOS Sourcerer API, schema",
        "abstract": {
          "@type": "vdoc:Chapter",
          "vdoc:content": [
            "This library provides the definitions and reference implementation\n    of the ValOS sourcerer architecture which is used to route ",
            {
              "@type": "vdoc:CharacterData",
              "vdoc:content": [
                "ValOS event streams"
              ]
            },
            "."
          ]
        },
        "introduction": {
          "@type": "vdoc:Chapter",
          "vdoc:content": []
        },
        "ontologyAbstract": {
          "vdoc:content": [
            "@valos/sourcerer ontology specifies the Valospace core types and\n      properties directly to the @valos/kernel namespace. "
          ]
        },
        "package": "@valos/sourcerer",
        "version": "0.35.0-prerelease.10"
      },
      "sourcerer/valos-event-log": {
        "@id": "https://valospace.org/sourcerer/valos-event-log",
        "tags": [],
        "subProfiles": [],
        "title": "ValOS Event Log",
        "abstract": {
          "@type": "vdoc:Chapter",
          "vdoc:content": [
            "ValOS Event Log is an ordered, numbered sequence of JSON-LD documents.\nEach document represents a single event. Together these events\nincrementally, exclusively and deterministically specify the state\nchanges of a single valospace partition from its initial empty state to\nthe current state after the most recent event."
          ]
        },
        "introduction": {
          "@type": "vdoc:Chapter",
          "vdoc:content": [
            "."
          ]
        },
        "package": "@valos/sourcerer",
        "version": "0.35.0-prerelease.10"
      },
      "twindoc": {
        "@id": "https://valospace.org/twindoc",
        "tags": [
          "PRIMARY",
          "ONTOLOGY"
        ],
        "subProfiles": [],
        "title": "TwinDoc - Valospace Hypertwin VDoc extension",
        "abstract": {
          "@type": "vdoc:Chapter",
          "vdoc:content": [
            "This document specifies TwinDoc, a ",
            {
              "@type": "vdoc:Reference",
              "vdoc:content": [
                "VDoc extension"
              ],
              "vdoc:ref": "@valos/vdoc#extension"
            },
            " which specifies an isomorphism and synchronization\n    transformations between VDoc documents and valospace resources.",
            null,
            "More specifically TwinDoc allows for the serialization and\n    deserialization of an arbitrary selection of valospace resources\n    into a VDoc document array and back even if the source resources\n    are not a representation of a VDoc document nor use any VDoc core\n    or extension ontologies."
          ]
        },
        "introduction": {
          "@type": "vdoc:Chapter",
          "vdoc:content": [
            "TwinDoc provides both full isomorphic synchronization as well as\n    incremental, additive updates between VDoc documents and valospace\n    resources.\n    The fully isomoprhic extraction and emission transformations to\n    valospace resources provide lossless roundtrips to both directions:",
            {
              "vdoc:content": [
                {
                  "@type": "vdoc:NumberedList",
                  "vdoc:entries": [
                    [
                      "emit + extract: a roundtrip starting from VDocLD into valospace back into VDocLD"
                    ],
                    [
                      "extract + emit: a roundtrip starting from valospace into VDocLD back into valospace"
                    ]
                  ]
                }
              ]
            },
            null,
            "TwinDoc also specifies incremental transformations which are given\n    a diff base in addition to the source and which compute a diffset\n    and then merge the resulting diffset to the pre-existing\n    transformation target.\n    This not only gives performance advantages but also makes it\n    possible to have the final document be a combination of several\n    partial primary sources."
          ]
        },
        "ontologyAbstract": {
          "vdoc:content": [
            "TwinDoc ontology provides vocabulary for defining hypertwin\n      mappings and configurations; actual hypertwin content is\n      represented using the valos core ontologies and possible\n      extension content ontologies."
          ]
        },
        "package": "@valos/twindoc",
        "version": "0.35.0-prerelease.10"
      },
      "type-vault/AssortedTutorials": {
        "@id": "https://valospace.org/type-vault/AssortedTutorials",
        "tags": [
          "PRIMARY",
          "HOW_TO"
        ],
        "subProfiles": [],
        "title": "Assorted tutorials",
        "abstract": {
          "@type": "vdoc:Chapter",
          "vdoc:content": [
            "This document is a collection of tutorials and possibly other notes",
            " created by Jaradacl based on the tasks given. (During first few days at least)"
          ]
        },
        "package": "@valos/type-vault",
        "version": "0.35.0-prerelease.10"
      },
      "vdoc": {
        "@id": "https://valospace.org/vdoc",
        "tags": [
          "PRIMARY",
          "ONTOLOGY"
        ],
        "subProfiles": [],
        "title": "VDoc - ValOS document interchange specification",
        "abstract": {
          "@type": "vdoc:Chapter",
          "vdoc:content": [
            "This document specifies VDoc, a ",
            {
              "@type": "vdoc:Reference",
              "vdoc:content": [
                "a JSON-LD"
              ],
              "vdoc:ref": "https://www.w3.org/TR/json-ld11/"
            },
            "-based documentation human-machine-valospace interchange format."
          ]
        },
        "introduction": {
          "@type": "vdoc:Chapter",
          "vdoc:content": [
            {
              "revdoc:dfn": "#vdoc",
              "vdoc:content": [
                {
                  "vdoc:strong": true,
                  "vdoc:content": [
                    {
                      "@type": "vdoc:Reference",
                      "vdoc:content": [
                        "VDoc"
                      ],
                      "vdoc:ref": "#vdoc"
                    }
                  ]
                },
                " is an extensible JSON-LD interchange\n      specification for extracting documents from varying sources,\n      passing the now-machine-manipulable interchange document around\n      and subsequently producing documents of specific formats such\n      as Valospace resources, markdown, ReSpec HTML and browser and\n      ansi-colored console outputs."
              ]
            },
            null,
            "Motivation for this specification is to provide the foundation\n    for document ",
            {
              "@type": "vdoc:Reference",
              "vdoc:content": [
                "Valospace hypertwins"
              ],
              "vdoc:ref": "@valos/hypertwin"
            },
            " by supporting the ValOS resources as an emission target. This\n    allows all kinds of documents to be accessible from within\n    Valospace with minimal additional tooling. This is not made\n    an explicit design goal unto itself; instead the design goals are\n    chosen to be generic in a way that satisfies this goal as the\n    original author believes this leads to better design."
          ]
        },
        "ontologyAbstract": {
          "vdoc:content": [
            "VDoc core ontology specifies the vocabulary for the human facing\n      document structure by means of primitives which are sufficiently\n      common and meaningful across all types of documents.\n      These primitives include constructs such as chapters, titles,\n      lists, tables, cross-references, etc.",
            "VDoc core ontology explicitly does not specify any semantic\n      meanings outside the document structure itself."
          ]
        },
        "package": "@valos/vdoc",
        "version": "0.35.0-prerelease.10"
      },
      "kernel": {
        "@id": "https://valospace.org/kernel",
        "tags": [
          "PRIMARY",
          "DOMAIN",
          "ONTOLOGY",
          "TECHNICIAN"
        ],
        "subProfiles": [],
        "title": "@valos/kernel domain content reference",
        "abstract": {
          "@type": "vdoc:Chapter",
          "vdoc:content": [
            "@valos/kernel domain ",
            "includes all core infrastructure components of ValOS - the Valaa Open System.",
            null,
            "These components are hosted at the ",
            {
              "@type": "vdoc:Reference",
              "vdoc:content": [
                "npmjs repository within @valos namespace"
              ],
              "vdoc:ref": "https://www.npmjs.com/search?q=%40valos"
            },
            ".",
            null,
            "These components are developed at the ",
            {
              "@type": "vdoc:Reference",
              "vdoc:content": [
                "valos git repository"
              ],
              "vdoc:ref": "https://github.com/valaatech/kernel"
            },
            "."
          ]
        },
        "introduction": {
          "@type": "vdoc:Chapter",
          "vdoc:content": [
            "ValOS ecosystem revolves around various roles. This document is\n      a reference document of the ValOS fabric systems and structures\n      and is directed for technicians. Check out the brief\n      description and introductions of the other roles as well.",
            null,
            {
              "@type": "vdoc:Reference",
              "vdoc:content": [
                "Valma"
              ],
              "vdoc:ref": "Valma"
            },
            " itself is a collection of tools for interacting\n      with the ValOS ecosystem, most notable of which is ",
            {
              "@type": "vdoc:Reference",
              "vdoc:content": [
                [
                  {
                    "vdoc:em": true,
                    "vdoc:content": [
                      "vlm"
                    ]
                  },
                  " the command line script invoker"
                ]
              ],
              "vdoc:ref": "@/valma"
            },
            ".",
            {
              "vdoc:lookup": "documents",
              "@type": "vdoc:Table",
              "vdoc:headers": {
                "vdoc:entries": [
                  {
                    "@type": "vdoc:Header",
                    "vdoc:cell": {
                      "vdoc:strong": true,
                      "vdoc:content": [
                        {
                          "@type": "vdoc:Reference",
                          "vdoc:content": [
                            "vdoc:selectKey"
                          ],
                          "vdoc:ref": "vdoc:selectKey"
                        }
                      ]
                    },
                    "vdoc:content": [
                      "Your role:"
                    ]
                  },
                  {
                    "@type": "vdoc:Header",
                    "vdoc:cell": {
                      "vdoc:strong": true,
                      "vdoc:content": [
                        {
                          "vdoc:em": true,
                          "vdoc:content": [
                            {
                              "@type": "vdoc:Reference",
                              "vdoc:content": [
                                {
                                  "vdoc:selectField": "title"
                                }
                              ],
                              "vdoc:ref": [
                                "vdoc:selectKey",
                                "#introduction"
                              ]
                            }
                          ]
                        }
                      ]
                    },
                    "vdoc:content": [
                      "Your answer..."
                    ]
                  },
                  {
                    "vdoc:cell": "introduction",
                    "@type": "vdoc:Header",
                    "vdoc:content": {
                      "vdoc:em": true,
                      "vdoc:content": [
                        "Introduction:"
                      ]
                    },
                    "vdoc:wide": true,
                    "vdoc:tall": true
                  },
                  {
                    "@type": "vdoc:Header",
                    "vdoc:content": {
                      "vdoc:em": true,
                      "vdoc:content": [
                        "Aliases:"
                      ]
                    },
                    "vdoc:wide": true,
                    "vdoc:cell": {
                      "vdoc:em": true,
                      "vdoc:content": [
                        {
                          "@type": "vdoc:Reference",
                          "vdoc:content": [
                            {
                              "vdoc:words": {
                                "vdoc:selectField": "subProfiles"
                              }
                            }
                          ],
                          "vdoc:ref": [
                            "vdoc:selectKey",
                            "#section_profiles"
                          ]
                        }
                      ]
                    }
                  }
                ]
              },
              "vdoc:entries": [
                "technician",
                "valonaut",
                "voyager"
              ]
            }
          ]
        },
        "ontologyAbstract": {
          "vdoc:content": [
            "@valos/kernel ontology provides vocabulary and definitions of\n      the ValOS core concepts."
          ]
        },
        "package": "@valos/kernel",
        "version": "0.35.0-prerelease.10"
      },
      "@valos/kernel": {
        "@id": "https://valospace.org/index",
        "tags": [
          "PRIMARY",
          "INTRODUCTION",
          "ONTOLOGY",
          "VALONAUT"
        ],
        "subProfiles": [],
        "title": "Valospace reference",
        "abstract": {
          "@type": "vdoc:Chapter",
          "vdoc:content": [
            "Overview of the valospace APIs and ontologies."
          ]
        },
        "introduction": {
          "@type": "vdoc:Chapter",
          "vdoc:content": [
            "ValOS ecosystem revolves around various roles. This document\n      is a reference document of valospace systems and structures and\n      is directed for more experienced valonauts. Check out the brief\n      description and introductions of the other roles as well.",
            null,
            ".",
            {
              "vdoc:lookup": "documents",
              "@type": "vdoc:Table",
              "vdoc:headers": {
                "vdoc:entries": [
                  {
                    "@type": "vdoc:Header",
                    "vdoc:cell": {
                      "vdoc:strong": true,
                      "vdoc:content": [
                        {
                          "@type": "vdoc:Reference",
                          "vdoc:content": [
                            "vdoc:selectKey"
                          ],
                          "vdoc:ref": "vdoc:selectKey"
                        }
                      ]
                    },
                    "vdoc:content": [
                      "Your role:"
                    ]
                  },
                  {
                    "@type": "vdoc:Header",
                    "vdoc:cell": {
                      "vdoc:strong": true,
                      "vdoc:content": [
                        {
                          "vdoc:em": true,
                          "vdoc:content": [
                            {
                              "@type": "vdoc:Reference",
                              "vdoc:content": [
                                {
                                  "vdoc:selectField": "title"
                                }
                              ],
                              "vdoc:ref": [
                                "vdoc:selectKey",
                                "#introduction"
                              ]
                            }
                          ]
                        }
                      ]
                    },
                    "vdoc:content": [
                      "Your answer..."
                    ]
                  },
                  {
                    "vdoc:cell": "introduction",
                    "@type": "vdoc:Header",
                    "vdoc:content": {
                      "vdoc:em": true,
                      "vdoc:content": [
                        "Introduction:"
                      ]
                    },
                    "vdoc:wide": true,
                    "vdoc:tall": true
                  },
                  {
                    "@type": "vdoc:Header",
                    "vdoc:content": {
                      "vdoc:em": true,
                      "vdoc:content": [
                        "Aliases:"
                      ]
                    },
                    "vdoc:wide": true,
                    "vdoc:cell": {
                      "vdoc:em": true,
                      "vdoc:content": [
                        {
                          "@type": "vdoc:Reference",
                          "vdoc:content": [
                            {
                              "vdoc:words": {
                                "vdoc:selectField": "subProfiles"
                              }
                            }
                          ],
                          "vdoc:ref": [
                            "vdoc:selectKey",
                            "#section_profiles"
                          ]
                        }
                      ]
                    }
                  }
                ]
              },
              "vdoc:entries": [
                "technician",
                "valonaut",
                "voyager"
              ]
            }
          ]
        },
        "ontologyAbstract": {
          "vdoc:content": [
            "Valospace ontology provides vocabulary and definitions of\n      the primary ValOS resources."
          ]
        },
        "package": "@valos/kernel",
        "version": "0.35.0-prerelease.10"
      },
      "technician": {
        "@id": "https://valospace.org/technician",
        "tags": [
          "PRIMARY",
          "ROLE"
        ],
        "subProfiles": [
          "contributor",
          "developer",
          "administrator",
          "devops",
          "hacker",
          "etc"
        ],
        "title": "\"I am a ValOS technician, I want to enable valonauts and expand valospace\"",
        "abstract": {
          "@type": "vdoc:Chapter",
          "vdoc:content": [
            "This document is the first introduction for ValOS technicians -\n    the primary infrastructure developers and operators - to the ValOS\n    ecosystem and its infrastructure toolchains and workflows."
          ]
        },
        "introduction": {
          "@type": "vdoc:Chapter",
          "vdoc:content": [
            "As a technician you develop and operate the ",
            {
              "revdoc:dfn": "#fabric",
              "vdoc:content": [
                {
                  "vdoc:strong": true,
                  "vdoc:content": [
                    {
                      "@type": "vdoc:Reference",
                      "vdoc:content": [
                        "ValOS fabric"
                      ],
                      "vdoc:ref": "#fabric"
                    }
                  ]
                },
                ", ",
                "the globally distributed web-like infrastructure of servers,\n        services and components which underlies the Valospace"
              ]
            },
            ".",
            null,
            "    You use ",
            {
              "@type": "vdoc:Reference",
              "vdoc:content": [
                "vlm"
              ],
              "vdoc:ref": "@/valma"
            },
            " and employ your existing,\n    likely professional knowledge of JavaScript, Node.js, DevOps,\n    backend, library and other software development skills.",
            null,
            "    You create new open source and/or proprietary node packages. These\n    permanently create new fabric functionalities and ",
            {
              "@type": "vdoc:Reference",
              "vdoc:content": [
                "expand"
              ],
              "vdoc:ref": "expand"
            },
            " the Valospace by integrating it to old world systems."
          ]
        },
        "package": "@valos/kernel",
        "version": "0.35.0-prerelease.10"
      },
      "valonaut": {
        "@id": "https://valospace.org/valonaut",
        "tags": [
          "PRIMARY",
          "ROLE"
        ],
        "subProfiles": [
          "everyone",
          "personal",
          "student",
          "prototypist",
          "etc"
        ],
        "title": "\"I am a valonaut, I want to create and share interactive content\"",
        "abstract": {
          "@type": "vdoc:Chapter",
          "vdoc:content": [
            "This document is the first introduction for valonauts - the\n    primary content creators - to the ValOS ecosystem and its core\n    tools."
          ]
        },
        "introduction": {
          "@type": "vdoc:Chapter",
          "vdoc:content": [
            "As a valonaut you create, share and deploy web content and\n    interactive applications fully from inside ",
            {
              "@type": "vdoc:Reference",
              "vdoc:content": [
                "Valospace"
              ],
              "vdoc:ref": "Valospace"
            },
            ".",
            null,
            "You use a web editor called ",
            {
              "@type": "vdoc:Reference",
              "vdoc:content": [
                "Zero"
              ],
              "vdoc:ref": "Zero"
            },
            " and with it employ\n    traditional web technologies; HTML5, CSS and the Javascript\n    dialect ",
            {
              "@type": "vdoc:Reference",
              "vdoc:content": [
                "valoscript"
              ],
              "vdoc:ref": "@valos/script"
            },
            null,
            "The skills you learn to do this are like cycling or writing - they\n    are used to support your other interests. While you don't need to\n    become a professional you certainly can!"
          ]
        },
        "package": "@valos/kernel",
        "version": "0.35.0-prerelease.10"
      },
      "voyager": {
        "@id": "https://valospace.org/voyager",
        "tags": [
          "PRIMARY",
          "ROLE"
        ],
        "subProfiles": [
          "enthusiast",
          "entrepreneur",
          "evangelist",
          "investor",
          "business_owner",
          "sales_rep",
          "etc"
        ],
        "title": "\"I am a ValOS voyager, I want to discover ValOS and enlighten others\"",
        "abstract": {
          "@type": "vdoc:Chapter",
          "vdoc:content": [
            "This document is the first introduction for ValOS voyagers -\n    the first adopters, entrepreneurs and evangelists - to the ValOS\n    ecosystem, its philosophy and its ultimate goals."
          ]
        },
        "introduction": {
          "@type": "vdoc:Chapter",
          "vdoc:content": [
            "As a voyager you have stakes that matter. Whether you were to\n    invest on a ValOS collaborator as a financier, to adopt ValOS as\n    technology as an executive or just to commit your personal time and\n    energy on a ValOS project you need to ",
            {
              "vdoc:em": true,
              "vdoc:content": [
                "see"
              ]
            },
            " forward.",
            null,
            "To make sound decisions and to position yourself proactively you\n    need to understand the big picture and philosophy of the ValOS\n    ecosystem. Only then you can enlighten others.",
            null,
            "You use tailored but real-world ValOS demo setups to illustrate\n    how ValOS a solution could be configured to meet the needs at hand.\n    Your audience can be your customer, your team or even just\n    yourself."
          ]
        },
        "package": "@valos/kernel",
        "version": "0.35.0-prerelease.10"
      }
    },
    "prefixes": {
      "@id": "prefixes",
      "rdf": "http://www.w3.org/1999/02/22-rdf-syntax-ns#",
      "rdfs": "http://www.w3.org/2000/01/rdf-schema#",
      "xsd": "http://www.w3.org/2001/XMLSchema#",
      "owl": "http://www.w3.org/2002/07/owl#",
      "dc": "http://purl.org/dc/elements/1.1/",
      "valos-kernel": "https://valospace.org/kernel#",
      "valos": "https://valospace.org/#",
      "valos-raem": "https://valospace.org/raem#"
    },
    "vocabulary": {
      "@id": "vocabulary",
      "Resource": {
        "@type": "valos-raem:Type",
        "rdfs:subClassOf": "rdfs:Resource",
        "revdoc:brief": "valospace resource interface",
        "rdfs:comment": "The class of resources which can appear as a subject in valospace\nresource and event graphs. The domain of all transient and generated\nfields which are available even for unsourced bodies."
      },
      "id": {
        "@type": "valos-raem:GeneratedField",
        "rdfs:domain": "valos:Resource",
        "rdfs:range": "xsd:string",
        "restriction": {
          "@type": "owl:Restriction",
          "owl:cardinality": 1
        },
        "valos-raem:generator": "getId",
        "rdfs:comment": "The immutable resource id of this resource."
      },
      "iri": {
        "@type": "valos-raem:GeneratedField",
        "rdfs:domain": "valos:Resource",
        "rdfs:range": "xsd:anyURI",
        "restriction": {
          "@type": "owl:Restriction",
          "owl:cardinality": 1
        },
        "valos-raem:generator": "getIRI",
        "rdfs:comment": "The authoritative locator IRI of this resource in the current view of\nthe world. Always equivalent to a catenation of\n<valos:partitionIRI> \"#\" <valos:id>\nof this resource"
      },
      "rawId": {
        "@type": "valos-raem:AliasField",
        "revdoc:deprecatedInFavorOf": "valos:id",
        "valos-raem:aliasOf": "valos:id",
        "rdfs:subPropertyOf": "valos:id",
        "rdfs:domain": "valos:Resource",
        "rdfs:range": "xsd:string",
        "restriction": {
          "@type": "owl:Restriction",
          "owl:cardinality": 1
        },
        "valos-raem:generator": "getRawId",
        "rdfs:comment": "The resource id of this resource"
      },
      "typeName": {
        "@type": "valos-raem:GeneratedField",
        "rdfs:domain": "valos:Resource",
        "rdfs:range": "xsd:string",
        "restriction": {
          "@type": "owl:Restriction",
          "owl:cardinality": 1
        },
        "valos-raem:generator": "getTransientTypeName",
        "rdfs:comment": "The dominant type name of this resource"
      },
      "partition": {
        "@type": "valos-raem:GeneratedField",
        "rdfs:domain": "valos:Resource",
        "rdfs:range": "valos:Partition",
        "restriction": {
          "@type": "owl:Restriction",
          "owl:maxCardinality": 1
        },
        "valos-raem:generator": "partitionResolver",
        "rdfs:comment": "The partition root resource of this resource, ie. the nearest ancestor\n(possibly self) with a non-null valos:authorityIRI."
      },
      "partitionIRI": {
        "@type": "valos-raem:GeneratedField",
        "rdfs:domain": "valos:Resource",
        "rdfs:range": "xsd:anyURI",
        "restriction": {
          "@type": "owl:Restriction",
          "owl:maxCardinality": 1
        },
        "valos-raem:generator": "partitionURIResolver",
        "rdfs:comment": "The partition IRI of the partition this resource belongs to in the\ncurrent view of the world."
      },
      "partitionURI": {
        "@type": "valos-raem:AliasField",
        "revdoc:deprecatedInFavorOf": "valos:partitionIRI",
        "valos-raem:aliasOf": "valos:partitionIRI",
        "rdfs:subPropertyOf": "valos:partitionIRI",
        "rdfs:domain": "valos:Resource",
        "rdfs:range": "xsd:anyURI",
        "restriction": {
          "@type": "owl:Restriction",
          "owl:maxCardinality": 1
        }
      },
      "prototype": {
        "@type": "valos-raem:PrimaryField",
        "rdfs:domain": "valos:Resource",
        "rdfs:range": "valos:Resource",
        "restriction": {
          "@type": "owl:Restriction",
          "owl:maxCardinality": 1
        },
        "valos-raem:coupledField": "valos:derivations",
        "rdfs:comment": "The prototype of this resource. All field lookups for which there is\nno associated value set and whose field descriptors don't have\nownDefaultValue are forwarded to the prototype."
      },
      "derivations": {
        "@type": "valos-raem:TransientField",
        "rdfs:domain": "valos:Resource",
        "rdfs:range": "valos:Resource",
        "valos-raem:coupledField": "valos:prototype",
        "valos-raem:preventsDestroy": true,
        "valos-raem:ownDefaultValue": [],
        "rdfs:comment": "An unordered set of resources which have this resource as their\nvalos:prototype."
      },
      "ownFields": {
        "@type": "valos-raem:GeneratedField",
        "rdfs:domain": "valos:Resource",
        "rdfs:range": "valos:Resource",
        "restriction": {
          "@type": "owl:Restriction",
          "owl:maxCardinality": 1
        },
        "valos-raem:generator": "resolveOwnFields",
        "rdfs:comment": "A transient version of this object as if prototype was undefined.\nAll property accesses will only return field values which are directly\nowned by this resource."
      },
      "inheritancePrototype": {
        "@type": "valos-raem:PrimaryField",
        "rdfs:subPropertyOf": "valos:prototype",
        "rdfs:domain": "valos:Resource",
        "rdfs:range": "valos:Resource",
        "restriction": {
          "@type": "owl:Restriction",
          "owl:maxCardinality": 1
        },
        "valos-raem:coupledField": "valos:inheritors",
        "rdfs:comment": "The derivation prototype of this resource. This represents the\ntraditional prototypical inheritance where inherited field values are\nnot remapped in any way."
      },
      "inheritors": {
        "@type": "valos-raem:TransientField",
        "rdfs:subPropertyOf": "valos:derivations",
        "rdfs:domain": "valos:Resource",
        "rdfs:range": "valos:Resource",
        "valos-raem:coupledField": "valos:inheritancePrototype",
        "valos-raem:preventsDestroy": true,
        "valos-raem:ownDefaultValue": [],
        "rdfs:comment": "An unordered set of resources which have this resource as their\nvalos:inheritancePrototype."
      },
      "instancePrototype": {
        "@type": "valos-raem:PrimaryField",
        "rdfs:subPropertyOf": "valos:prototype",
        "rdfs:domain": "valos:Resource",
        "rdfs:range": "valos:Resource",
        "restriction": {
          "@type": "owl:Restriction",
          "owl:maxCardinality": 1
        },
        "valos-raem:coupledField": "valos:instances",
        "rdfs:comment": "The instance prototype of this resource instance."
      },
      "instances": {
        "@type": "valos-raem:TransientField",
        "rdfs:subPropertyOf": "valos:derivations",
        "rdfs:domain": "valos:Resource",
        "rdfs:range": "valos:Resource",
        "valos-raem:coupledField": "valos:instancePrototype",
        "valos-raem:preventsDestroy": true,
        "valos-raem:ownDefaultValue": [],
        "rdfs:comment": "An unordered set of resources which have this resource as their\ndirectvalospace:instancePrototype."
      },
      "ghostPrototype": {
        "@type": "valos-raem:GeneratedField",
        "rdfs:subPropertyOf": "valos:prototype",
        "rdfs:domain": "valos:Resource",
        "rdfs:range": "valos:Resource",
        "restriction": {
          "@type": "owl:Restriction",
          "owl:maxCardinality": 1
        },
        "valos-raem:generator": "ghostPrototypeResolver",
        "valos-raem:coupledField": "valos:ghosts",
        "rdfs:comment": "Ghost prototype of this ghost resource. The ghost prototype is the\nbase resource from which this ghost was created during some primary\ninstantiation.\nThis instantiation (which happens on prototype and results in an\ninstance of it) also ghost-instantiates all the direct and indirect\nownlings of the prototype as ghost ownlings in the instance. The\ninstance is called the *ghost host* of all these ghosts. Likewise, the\ninstance prototype is called the ghost host prototype, and the\n(grand-)ownlings of this ghost host prototype are the ghost prototypes\nof the corresponding ghosts (ie. this field).} ."
      },
      "ghosts": {
        "@type": "valos-raem:TransientField",
        "rdfs:subPropertyOf": "valos:derivations",
        "rdfs:domain": "valos:Resource",
        "rdfs:range": "valos:Resource",
        "valos-raem:coupledField": "valos:ghostPrototype",
        "valos-raem:preventsDestroy": true,
        "valos-raem:ownDefaultValue": [],
        "rdfs:comment": "An unordered set of all (materialized) ghosts which have this resource\nas their valos:ghostPrototype. See @valos/raem#section_ghost_instancing\nfor why immaterial ghosts are not listed."
      },
      "materializedGhosts": {
        "@type": "valos-raem:AliasField",
        "revdoc:deprecatedInFavorOf": "valos:ghosts",
        "valos-raem:aliasOf": "valos:ghosts",
        "rdfs:subPropertyOf": "valos:ghosts",
        "rdfs:domain": "valos:Resource",
        "rdfs:range": "valos:Resource",
        "valos-raem:coupledField": "valos:ghostPrototype",
        "valos-raem:preventsDestroy": true,
        "valos-raem:ownDefaultValue": []
      },
      "unnamedCouplings": {
        "@type": "valos-raem:TransientField",
        "rdfs:domain": "valos-raem:TransientField",
        "rdfs:range": "valos-raem:TransientField",
        "valos-raem:coupledField": "",
        "valos-raem:isOwnerOf": true,
        "rdfs:comment": "Referrers with a missing coupledField referring this resource"
      },
      "ghostHost": {
        "@type": "valos-raem:GeneratedField",
        "rdfs:domain": "valos:Resource",
        "rdfs:range": "valos:Resource",
        "restriction": {
          "@type": "owl:Restriction",
          "owl:maxCardinality": 1
        },
        "valos-raem:generator": "ghostHostResolver",
        "rdfs:comment": "The instance resource which brought this ghost into being. This\ninstance is equivalent to the innermost ancestor of this ghost which is\nnot a ghost itself."
      },
      "ghostOwner": {
        "@type": "valos-raem:TransientField",
        "rdfs:domain": "valos:Resource",
        "rdfs:range": "valos:Resource",
        "restriction": {
          "@type": "owl:Restriction",
          "owl:maxCardinality": 1
        },
        "valos-raem:coupledField": "valos:ghostOwnlings",
        "valos-raem:isOwnedBy": true,
        "valos-raem:ownDefaultValue": null,
        "valos-raem:allowTransientFieldToBeSingular": true,
        "rdfs:comment": "The instance resource which owns this materialized ghost or null if\nthis ghost is immaterial.\nNote that materialized ghosts will have a two own fields: the\nghostOwner and the regular owner (or one of its aliases). The\nremoval of either of these owning field relationships will\nimmaterialize, not destroy, the ghost."
      },
      "ghostOwnlings": {
        "@type": "valos-raem:TransientField",
        "rdfs:domain": "valos:Resource",
        "rdfs:range": "valos:Resource",
        "valos-raem:isOwnerOf": true,
        "valos-raem:coupledField": "valos:ghostOwner",
        "valos-raem:ownDefaultValue": [],
        "rdfs:comment": "Materialized ghost resources which have this instance as their ghost\nhost."
      },
      "Bvob": {
        "@type": "valos-raem:Type",
        "revdoc:brief": "Binary ValOS Object type",
        "rdfs:subClassOf": "valos:Resource",
        "rdfs:comment": "The dominant type class of resources which are immutably associated\nwith an octet-stream of fixed length. Bvob resources have a hash of\nthat octet-stream, prefixed with the hash algorithm, as their resource\nid."
      },
      "hashAlgorithm": {
        "@type": "valos-raem:GeneratedField",
        "rdfs:domain": "valos:Bvob",
        "rdfs:range": "xsd:string",
        "restriction": {
          "@type": "owl:Restriction",
          "owl:cardinality": 1
        },
        "valos-raem:generator": "hashAlgorithm",
        "rdfs:comment": "The hash algorithm used to create the content hash of this Bvob"
      },
      "contentHash": {
        "@type": "valos-raem:GeneratedField",
        "rdfs:domain": "valos:Bvob",
        "rdfs:range": "xsd:string",
        "restriction": {
          "@type": "owl:Restriction",
          "owl:cardinality": 1
        },
        "valos-raem:generator": "contentHash",
        "rdfs:comment": "The content hash of the octet-stream associated with this Bvob"
      },
      "contentLength": {
        "@type": "valos-raem:GeneratedField",
        "rdfs:domain": "valos:Bvob",
        "rdfs:range": "xsd:nonNegativeInteger",
        "restriction": {
          "@type": "owl:Restriction",
          "owl:cardinality": 1
        },
        "valos-raem:generator": "contentLength",
        "rdfs:comment": "The number of octets in the octet-stream associated with this Bvob."
      },
      "contentReferrers": {
        "@type": "valos-raem:TransientField",
        "rdfs:domain": "valos:Bvob",
        "rdfs:range": "valos:Sourced",
        "valos-raem:defaultCoupledField": "valos:content",
        "rdfs:comment": "The unordered set of valos:content references to this Bvob from\nwithin this view of the world."
      },
      "Sourced": {
        "@type": "valos-raem:Type",
        "rdfs:subClassOf": "valos:Resource",
        "revdoc:brief": "active, visible resource interface",
        "rdfs:comment": "The class of valospace resources that are sourced in this view of\nthe world. A sourced resource has all of its fields and properties\navailable and it can thus be manipulated."
      },
      "owner": {
        "@type": "valos-raem:PrimaryField",
        "rdfs:domain": "valos:Sourced",
        "rdfs:range": "valos:Sourced",
        "restriction": {
          "@type": "owl:Restriction",
          "owl:maxCardinality": 1
        },
        "valos-raem:isOwnedBy": true,
        "valos-raem:defaultCoupledField": "valos:ownlings",
        "rdfs:comment": "The owner of this resource"
      },
      "name": {
        "@type": "valos-raem:PrimaryField",
        "rdfs:domain": "valos:Sourced",
        "rdfs:range": "xsd:string",
        "restriction": {
          "@type": "owl:Restriction",
          "owl:maxCardinality": 1
        },
        "rdfs:comment": "The primary ValOS name of this resource. It is globally non-unique but\noften context-dependently unique."
      },
      "ownlings": {
        "@type": "valos-raem:PrimaryField",
        "rdfs:domain": "valos:Sourced",
        "rdfs:range": "rdfs:List",
        "valos-raem:isOwnerOf": true,
        "valos-raem:coupledField": "valos:owner",
        "rdfs:comment": "The ordered list of all resources owned by this resource. This\nlist is a union of all fields with a valos-raem:isOwnerOf in their\nontology definition."
      },
      "unnamedOwnlings": {
        "@type": "valos-raem:PrimaryField",
        "rdfs:subPropertyOf": "valos:ownlings",
        "rdfs:domain": "valos:Sourced",
        "rdfs:range": "valos:Sourced",
        "valos-raem:isOwnerOf": true,
        "valos-raem:coupledField": "valos:owner",
        "rdfs:comment": "The ordered list of all resources owned by this resource which are not\ncontained in another valos-raem:isOwnerOf field list."
      },
      "isFrozen": {
        "@type": "valos-raem:PrimaryField",
        "rdfs:domain": "valos:Sourced",
        "rdfs:range": "xsd:boolean",
        "restriction": {
          "@type": "owl:Restriction",
          "owl:cardinality": 1
        },
        "valos-raem:isDuplicateable": false,
        "valos-raem:ownDefaultValue": false,
        "rdfs:comment": "Indicates whether this resource is frozen. A frozen resource nor any\nof its ownlings cannot have any of their primary fields be modified.\nSetting isFrozen to true is (by design) an irreversible operation.\nIf this resource is also the root resource of a partition the whole\npartition is permanently frozen."
      },
      "Unsourced": {
        "@type": "valos-raem:Type",
        "rdfs:subClassOf": "valos:Resource",
        "revdoc:brief": "out-of-this-world resource type",
        "rdfs:comment": "The dominant type class of 'unsourced' valospace resources. An\nunsourced resource doesn't have a known representation in this view of\nthe world, typically because it is inside an unsourced Partition.\nThe transition from Unsourced to and from other dominant types is the\nonly possible runtime type change and happens dynamically based on\nthe partition sourcery and banishment."
      },
      "Destroyed": {
        "@type": "valos-raem:Type",
        "rdfs:subClassOf": "valos:Resource",
        "revdoc:brief:": "destroyed resource type",
        "rdfs:comment": "The dominant type class of resources which have been destroyed."
      },
      "Partition": {
        "@type": "valos-raem:Type",
        "rdfs:subClassOf": "valos:Sourced",
        "revdoc:brief": "a document, world subdivision interface",
        "rdfs:comment": "A Partition is a subdivision of the whole ValOS object space into\nsmaller recursive, individually sourcable wholes. The Partition\nimplementation contains resources either by direct or transitive\nownership. Each such contained resource also knows their containing\nPartition.\n\nTODO(iridian, 2019-08): Update outdated terminology in this comment.\n\nIn addition to the few direct member fields relating to snapshotting\nand event stream synchronization, the Partition resources serve as\na key latching point for external services.\n\nEach Partition object is managed by an authority, which performs\nconflict resolution, authorization and recording of incoming commands,\nconverting them into the truth event log for that particular Partition.\n\nThe Partition id is used by the query routers to globally locate the\nauthority responsible for any given Partition. Also, cross-partition\nresource references are implemented as Unsourced resource stubs, ie.\nobjects that only contain the resource id and its most recently known\npartition (which will retain the new owning Partition in a stub,\nenabling forwarding). Together these allow for any resource to always\nbe eventually locateable from anywhere."
      },
      "authorityIRI": {
        "@type": "valos-raem:PrimaryField",
        "rdfs:domain": "valos:Partition",
        "rdfs:range": "xsd:anyURI",
        "restriction": {
          "@type": "owl:Restriction",
          "owl:maxCardinality": 1
        },
        "valos-raem:isDuplicateable": false,
        "valos-raem:ownDefaultValue": null,
        "rdfs:comment": "The authority IRI of this resource. If this field is set it means that\nthis is an active partition root object. The partition IRI is generated\nas per the rules specified by the authority IRI schema."
      },
      "partitionAuthorityURI": {
        "@type": "valos-raem:AliasField",
        "revdoc:deprecatedInFavorOf": "valos:authorityIRI",
        "valos-raem:aliasOf": "valos:authorityIRI",
        "rdfs:subPropertyOf": "valos:authorityIRI",
        "rdfs:domain": "valos:Partition",
        "rdfs:range": "xsd:string",
        "restriction": {
          "@type": "owl:Restriction",
          "owl:maxCardinality": 1
        }
      },
      "nameAlias": {
        "@type": "valos-raem:AliasField",
        "valos-raem:aliasOf": "valos:name",
        "rdfs:subPropertyOf": "valos:name",
        "rdfs:domain": "valos:Sourced",
        "rdfs:range": "xsd:string",
        "restriction": {
          "@type": "owl:Restriction",
          "owl:maxCardinality": 1
        },
        "rdfs:comment": "The primary name of this resource. It is globally non-unique but often\n  context-dependently unique.\n  This is an alias of valos:name for circumventing conflicts with the\n  native javascript property 'name' in some execution contexts"
      },
      "prototypeAlias": {
        "@type": "valos-raem:AliasField",
        "valos-raem:aliasOf": "valos:prototype",
        "rdfs:subPropertyOf": "valos:prototype",
        "rdfs:domain": "valos:Resource",
        "rdfs:range": "valos:Resource",
        "restriction": {
          "@type": "owl:Restriction",
          "owl:maxCardinality": 1
        },
        "rdfs:comment": "The prototype of this resource. This is an alias for valos:prototype\nto bypass conflicts with native javascript property 'prototype' in\ncertain contexts."
      },
      "ScriptResource": {
        "@type": "valos-raem:Type",
        "rdfs:subClassOf": [
          "valos:Resource"
        ],
        "revdoc:brief": "valoscript resource interface",
        "rdfs:comment": "The class of valospace resources which have script references to them\nfrom within this world. The domain of all transient and generated\nfields which are available even for out-of-this-world resources."
      },
      "incomingRelations": {
        "@type": "valos-raem:TransientField",
        "rdfs:domain": "valos:ScriptResource",
        "rdfs:range": "valos:Relation",
        "valos-raem:coupledField": "valos:target",
        "rdfs:comment": "The unordered set of relations that are targeting this relatable\nresource within this view of the world."
      },
      "ScriptDestroyed": {
        "@type": "valos-raem:Type",
        "rdfs:subClassOf": [
          "valos:Resource",
          "valos:ScriptResource"
        ],
        "revdoc:brief": "destroyed script resource type",
        "rdfs:comment": "The class of valospace script resources which have been destroyed in\nthis view of the world. It only provides the external fields listed in\nTransientScripFields and TransientFields interfaces."
      },
      "ScopeProperty": {
        "@type": "valos-raem:Type",
        "rdfs:subClassOf": [
          "valos:Resource",
          "valos:Sourced",
          "rdf:Statement"
        ],
        "revdoc:brief": "valoscript property",
        "rdfs:comment": "The class of valospace Property resources which belong to a scope."
      },
      "scope": {
        "@type": "valos-raem:AliasField",
        "valos-raem:aliasOf": "valos:owner",
        "rdfs:subPropertyOf": "valos:owner",
        "rdfs:domain": "valos:ScopeProperty",
        "rdfs:range": "valos:Scope",
        "restriction": {
          "@type": "owl:Restriction",
          "owl:maxCardinality": 1
        },
        "valos-raem:isOwnedBy": true,
        "valos-raem:coupledField": "valos:properties",
        "rdfs:comment": "The scope resource (and owner) of this ScopeProperty"
      },
      "value": {
        "@type": "valos-raem:PrimaryField",
        "rdfs:domain": "valos:ScopeProperty",
        "rdfs:range": "rdfs:Resource",
        "restriction": {
          "@type": "owl:Restriction",
          "owl:maxCardinality": 1
        },
        "valos-raem:initialValue": null,
        "valos-raem:finalDefaultValue": [
          "§void"
        ],
        "rdfs:comment": "The value of this ScopeProperty"
      },
      "twinspace": {
        "@type": "valos-raem:GeneratedField",
        "rdfs:domain": "valos:ScopeProperty",
        "rdfs:range": "rdfs:Resource",
        "restriction": {
          "@type": "owl:Restriction",
          "owl:maxCardinality": 1
        },
        "valos-raem:generator": "getTwinspace",
        "rdfs:comment": "The twinspace of this ScopeProperty. Equates to the expanded prefix\nof the valos:name of this ScopeProperty using the context of this\npartition. Additionally if the local part of the valos:name is an empty\nstring then the valos:value of this ScopeProperty defines\nthe twinspace id of the scope resource for this twinspace."
      },
      "subject": {
        "@type": "valos-raem:GeneratedField",
        "rdfs:subPropertyOf": "rdf:subject",
        "rdfs:domain": "valos:ScopeProperty",
        "rdfs:range": "rdfs:Resource",
        "restriction": {
          "@type": "owl:Restriction",
          "owl:maxCardinality": 1
        },
        "valos-raem:generator": "getSubject",
        "rdfs:comment": "The subject of this ScopeProperty when interpreted as a reified\nrdf:Statement. Equates to the twinspace id of the scope resource using\nthe valos:twinspace of this ScopeProperty."
      },
      "predicate": {
        "@type": "valos-raem:GeneratedField",
        "rdfs:subPropertyOf": "rdf:predicate",
        "rdfs:domain": "valos:ScopeProperty",
        "rdfs:range": "rdfs:Resource",
        "restriction": {
          "@type": "owl:Restriction",
          "owl:maxCardinality": 1
        },
        "valos-raem:generator": "getPredicate",
        "rdfs:comment": "The subject of this ScopeProperty when interpreted as a reified\nrdf:Statement. Equates to the IRI expansion of valos:name of this\nScopeProperty using the context of this partition."
      },
      "object": {
        "@type": "valos-raem:AliasField",
        "valos-raem:aliasOf": "valos:value",
        "rdfs:subPropertyOf": "rdf:object",
        "rdfs:domain": "valos:ScopeProperty",
        "rdfs:range": "rdfs:Resource",
        "restriction": {
          "@type": "owl:Restriction",
          "owl:maxCardinality": 1
        },
        "rdfs:comment": "The subject of this ScopeProperty when interpreted as a reified\nrdf:Statement. Equates to the twinspace id of the valos:value using\nthe valos:twinspace of this ScopeProperty if one is defined. Otherwise\nequals to the valos:value itself.\n"
      },
      "Scope": {
        "@type": "valos-raem:Type",
        "rdfs:subClassOf": [
          "valos:Resource"
        ],
        "revdoc:brief": "property namespace interface",
        "rdfs:comment": "The class of valospace resources which can have valoscript properties."
      },
      "properties": {
        "@type": "valos-raem:PrimaryField",
        "rdfs:domain": "valos:Scope",
        "rdfs:range": "rdfs:List",
        "valos-raem:coupledField": "valos:scope",
        "valos-raem:isOwnerOf": true,
        "rdfs:comment": "The ordered list of Property resources of this scope"
      },
      "Relatable": {
        "@type": "valos-raem:Type",
        "rdfs:subClassOf": [
          "valos:Resource",
          "valos:Sourced",
          "valos:ScriptResource",
          "valos:Scope"
        ],
        "revdoc:brief": "relation source and/or target interface",
        "rdfs:comment": "The class of valospace resources which can act as source and target of\na valospace Relation."
      },
      "relations": {
        "@type": "valos-raem:PrimaryField",
        "rdfs:domain": "valos:Relatable",
        "rdfs:range": "rdfs:List",
        "valos-raem:coupledField": "valos:source",
        "valos-raem:isOwnerOf": true,
        "rdfs:comment": "The ordered list of outgoing relations of this relatable"
      },
      "Relation": {
        "@type": "valos-raem:Type",
        "rdfs:subClassOf": [
          "valos:Resource",
          "valos:Sourced",
          "valos:ScriptResource",
          "valos:Scope",
          "valos:Relatable"
        ],
        "revdoc:brief": "primary directed relationship edge type",
        "rdfs:comment": "The class of valospace resources which represent directed,\nmany-to-many relationships between relatable resources.\nWith Entity and Media it forms the group of three primary types.\nAs a Scope it can have scriptable properties. Relation being\na Relatable itself allows for nested and recursive relationship\nstructures."
      },
      "source": {
        "@type": "valos-raem:AliasField",
        "valos-raem:aliasOf": "valos:owner",
        "rdfs:subPropertyOf": [
          "valos:owner",
          "rdf:source"
        ],
        "rdfs:domain": "valos:Relation",
        "rdfs:range": "valos:Relatable",
        "restriction": {
          "@type": "owl:Restriction",
          "owl:maxCardinality": 1
        },
        "valos-raem:isOwnedBy": true,
        "valos-raem:coupledField": "valos:relations",
        "rdfs:comment": "The source (and owner) relatable of this relation."
      },
      "target": {
        "@type": "valos-raem:PrimaryField",
        "rdfs:subPropertyOf": "rdf:object",
        "rdfs:domain": "valos:Relation",
        "rdfs:range": "valos:Relatable",
        "restriction": {
          "@type": "owl:Restriction",
          "owl:maxCardinality": 1
        },
        "valos-raem:coupledField": "valos:incomingRelations",
        "rdfs:comment": "The target relatable of this relation."
      },
      "directory": {
        "@type": "valos-raem:AliasField",
        "valos-raem:aliasOf": "valos:owner",
        "rdfs:subPropertyOf": "valos:owner",
        "rdfs:domain": [
          "valos:Entity",
          "valos:Media"
        ],
        "rdfs:range": "rdfs:Relatable",
        "restriction": {
          "@type": "owl:Restriction",
          "owl:maxCardinality": 1
        },
        "valos-raem:isOwnedBy": true,
        "valos-raem:coupledField": "valos:entries",
        "rdfs:comment": "The directory (and owner) relatable of this entry resource."
      },
      "entries": {
        "@type": "valos-raem:AliasField",
        "valos-raem:aliasOf": "valos:ownlings",
        "rdfs:subPropertyOf": "valos:ownlings",
        "rdfs:domain": "valos:Relatable",
        "rdfs:range": "rdfs:List",
        "valos-raem:isOwnerOf": true,
        "valos-raem:coupledField": "valos:directory",
        "rdfs:comment": "The ordered list of entry entities and medias of this relatable."
      },
      "Entity": {
        "@type": "valos-raem:Type",
        "revdoc:brief": "primary resource hierachy node type",
        "rdfs:subClassOf": [
          "valos:Resource",
          "valos:Sourced",
          "valos:ScriptResource",
          "valos:Scope",
          "valos:Relatable",
          "valos:Partition"
        ],
        "rdfs:comment": "The class of valospace resources which act as the main valospace\nhierarchy building block. With Relation and Media it forms the group of\nthree primary types. As a Scope it can have scriptable properties,\nwhich entities expose to all child resources as their lexical scripting\nnamespace.\n"
      },
      "parent": {
        "@type": "valos-raem:AliasField",
        "valos-raem:aliasOf": "valos:directory",
        "rdfs:subPropertyOf": "valos:directory",
        "rdfs:domain": "valos:Entity",
        "rdfs:range": "valos:Relatable",
        "restriction": {
          "@type": "owl:Restriction",
          "owl:maxCardinality": 1
        },
        "valos-raem:isOwnedBy": true,
        "valos-raem:coupledField": "valos:children",
        "rdfs:comment": "The parent (and owner) relatable of this entity."
      },
      "children": {
        "@type": "valos-raem:AliasField",
        "valos-raem:aliasOf": "valos:entries",
        "rdfs:subPropertyOf": "valos:entries",
        "rdfs:domain": "valos:Relatable",
        "rdfs:range": "rdfs:List",
        "valos-raem:isOwnerOf": true,
        "valos-raem:coupledField": "valos:parent",
        "rdfs:comment": "The ordered list of child entities of this relatable"
      },
      "Media": {
        "@type": "valos-raem:Type",
        "rdfs:subClassOf": [
          "valos:Resource",
          "valos:Sourced",
          "valos:ScriptResource",
          "valos:Scope",
          "valos:Relatable"
        ],
        "revdoc:brief": "primary file media type",
        "rdfs:comment": "The class of valospace resources which represent interpretable media\nand can be associated with mutable binary content and accompanying\nmetadata. With Relation and Media it forms the group of three primary\ntypes.\n"
      },
      "container": {
        "@type": "valos-raem:AliasField",
        "valos-raem:aliasOf": "valos:owner",
        "rdfs:subPropertyOf": "valos:owner",
        "rdfs:domain": "valos:Media",
        "rdfs:range": "valos:Relatable",
        "restriction": {
          "@type": "owl:Restriction",
          "owl:maxCardinality": 1
        },
        "valos-raem:isOwnedBy": true,
        "valos-raem:coupledField": "valos:medias",
        "rdfs:comment": "The container (and owner) relatable of this media."
      },
      "medias": {
        "@type": "valos-raem:AliasField",
        "valos-raem:aliasOf": "valos:ownlings",
        "rdfs:subPropertyOf": "valos:ownlings",
        "rdfs:domain": "valos:Relatable",
        "rdfs:range": "rdfs:List",
        "valos-raem:isOwnerOf": true,
        "valos-raem:coupledField": "valos:container",
        "rdfs:comment": "The ordered list of medias contained in this relatable"
      },
      "sourceURL": {
        "@type": "valos-raem:PrimaryField",
        "rdfs:domain": "valos:Media",
        "rdfs:range": "xsd:anyURI",
        "restriction": {
          "@type": "owl:Restriction",
          "owl:maxCardinality": 1
        },
        "rdfs:comment": "The unreliable source URL of this Media. This URL is dereferenced\nwhen the Media content is accessed and as such is subject to all\nfailure considerations associated with its protocol."
      },
      "content": {
        "@type": "valos-raem:PrimaryField",
        "rdfs:subPropertyOf": "rdf:object",
        "rdfs:domain": "valos:Media",
        "rdfs:range": "valos:Bvob",
        "restriction": {
          "@type": "owl:Restriction",
          "owl:maxCardinality": 1
        },
        "valos-raem:coupledField": "valos:contentReferrers",
        "rdfs:comment": "The infrastructure-backed octet-stream content of this Media."
      },
      "created": {
        "@type": "valos-raem:GeneratedField",
        "rdfs:domain": "valos:Media",
        "rdfs:range": "xsd:double",
        "restriction": {
          "@type": "owl:Restriction",
          "owl:maxCardinality": 1
        },
        "valos-raem:generator": "created",
        "rdfs:comment": "The creation UNIX epoch time of this Media. This is defined as the\ntruth log aspect timestamp of the CREATED event which brought this\nMedia into being."
      },
      "modified": {
        "@type": "valos-raem:GeneratedField",
        "rdfs:domain": "valos:Media",
        "rdfs:range": "xsd:double",
        "restriction": {
          "@type": "owl:Restriction",
          "owl:maxCardinality": 1
        },
        "valos-raem:generator": "modified",
        "rdfs:comment": "The latest modification UNIX epoch time of this Media. This is defined\nas the truth log aspect timestamp of the most recent event that\ndirectly affects this Media resource."
      }
    },
    "context": {
      "@id": "context",
      "restriction": {
        "@reverse": "owl:onProperty"
      },
      "valos:partition": {
        "@id": "https://valospace.org/#partition",
        "@type": "@id"
      },
      "valos:prototype": {
        "@id": "https://valospace.org/#prototype",
        "@type": "@id"
      },
      "valos:derivations": {
        "@id": "https://valospace.org/#derivations",
        "@type": "@id"
      },
      "valos:ownFields": {
        "@id": "https://valospace.org/#ownFields",
        "@type": "@id"
      },
      "valos:inheritancePrototype": {
        "@id": "https://valospace.org/#inheritancePrototype",
        "@type": "@id"
      },
      "valos:inheritors": {
        "@id": "https://valospace.org/#inheritors",
        "@type": "@id"
      },
      "valos:instancePrototype": {
        "@id": "https://valospace.org/#instancePrototype",
        "@type": "@id"
      },
      "valos:instances": {
        "@id": "https://valospace.org/#instances",
        "@type": "@id"
      },
      "valos:ghostPrototype": {
        "@id": "https://valospace.org/#ghostPrototype",
        "@type": "@id"
      },
      "valos:ghosts": {
        "@id": "https://valospace.org/#ghosts",
        "@type": "@id"
      },
      "valos:materializedGhosts": {
        "@id": "https://valospace.org/#materializedGhosts",
        "@type": "@id"
      },
      "valos:unnamedCouplings": {
        "@id": "https://valospace.org/#unnamedCouplings",
        "@type": "@id"
      },
      "valos:ghostHost": {
        "@id": "https://valospace.org/#ghostHost",
        "@type": "@id"
      },
      "valos:ghostOwner": {
        "@id": "https://valospace.org/#ghostOwner",
        "@type": "@id"
      },
      "valos:ghostOwnlings": {
        "@id": "https://valospace.org/#ghostOwnlings",
        "@type": "@id"
      },
      "valos:contentReferrers": {
        "@id": "https://valospace.org/#contentReferrers",
        "@type": "@id"
      },
      "valos:owner": {
        "@id": "https://valospace.org/#owner",
        "@type": "@id"
      },
      "valos:ownlings": {
        "@id": "https://valospace.org/#ownlings",
        "@container": "@list",
        "@type": "@id"
      },
      "valos:unnamedOwnlings": {
        "@id": "https://valospace.org/#unnamedOwnlings",
        "@type": "@id"
      },
      "valos:prototypeAlias": {
        "@id": "https://valospace.org/#prototypeAlias",
        "@type": "@id"
      },
      "valos:incomingRelations": {
        "@id": "https://valospace.org/#incomingRelations",
        "@type": "@id"
      },
      "valos:scope": {
        "@id": "https://valospace.org/#scope",
        "@type": "@id"
      },
      "valos:properties": {
        "@id": "https://valospace.org/#properties",
        "@container": "@list",
        "@type": "@id"
      },
      "valos:relations": {
        "@id": "https://valospace.org/#relations",
        "@container": "@list",
        "@type": "@id"
      },
      "valos:source": {
        "@id": "https://valospace.org/#source",
        "@type": "@id"
      },
      "valos:target": {
        "@id": "https://valospace.org/#target",
        "@type": "@id"
      },
      "valos:directory": {
        "@id": "https://valospace.org/#directory",
        "@type": "@id"
      },
      "valos:entries": {
        "@id": "https://valospace.org/#entries",
        "@container": "@list",
        "@type": "@id"
      },
      "valos:parent": {
        "@id": "https://valospace.org/#parent",
        "@type": "@id"
      },
      "valos:children": {
        "@id": "https://valospace.org/#children",
        "@container": "@list",
        "@type": "@id"
      },
      "valos:container": {
        "@id": "https://valospace.org/#container",
        "@type": "@id"
      },
      "valos:medias": {
        "@id": "https://valospace.org/#medias",
        "@container": "@list",
        "@type": "@id"
      },
      "valos:content": {
        "@id": "https://valospace.org/#content",
        "@type": "@id"
      }
    },
    "abstract": {
      "@id": "abstract",
      "@type": "vdoc:Chapter",
      "vdoc:content": [
        "Overview of the valospace APIs and ontologies."
      ]
    },
    "sotd": {
      "@id": "sotd",
      "@type": "vdoc:Chapter",
      "vdoc:content": [
        "This document is part of the vault workspace ",
        {
          "@type": "revdoc:Package",
          "vdoc:content": [
            {
              "vdoc:em": true,
              "vdoc:content": [
                "@valos/kernel"
              ]
            }
          ],
          "vdoc:ref": "@valos/kernel"
        },
        " (of domain ",
        {
          "@type": "revdoc:Package",
          "vdoc:content": [
            {
              "vdoc:em": true,
              "vdoc:content": [
                "@valos/kernel"
              ]
            }
          ],
          "vdoc:ref": "@valos/kernel"
        },
        ") which is ",
        "ValOS common infrastructure tools and libraries monorepository."
      ]
    },
    "introduction": {
      "@id": "introduction",
      "@type": "vdoc:Chapter",
      "dc:title": {
        "vdoc:em": true,
        "vdoc:content": [
          "\"Greetings, I am Valma, the ValOS Mediator. Who are you?\""
        ]
      },
      "vdoc:content": [
        "ValOS ecosystem revolves around various roles. This document\n      is a reference document of valospace systems and structures and\n      is directed for more experienced valonauts. Check out the brief\n      description and introductions of the other roles as well.",
        null,
        ".",
        {
          "vdoc:lookup": "documents",
          "@type": "vdoc:Table",
          "vdoc:headers": {
            "vdoc:entries": [
              {
                "@type": "vdoc:Header",
                "vdoc:cell": {
                  "vdoc:strong": true,
                  "vdoc:content": [
                    {
                      "@type": "vdoc:Reference",
                      "vdoc:content": [
                        "vdoc:selectKey"
                      ],
                      "vdoc:ref": "vdoc:selectKey"
                    }
                  ]
                },
                "vdoc:content": [
                  "Your role:"
                ]
              },
              {
                "@type": "vdoc:Header",
                "vdoc:cell": {
                  "vdoc:strong": true,
                  "vdoc:content": [
                    {
                      "vdoc:em": true,
                      "vdoc:content": [
                        {
                          "@type": "vdoc:Reference",
                          "vdoc:content": [
                            {
                              "vdoc:selectField": "title"
                            }
                          ],
                          "vdoc:ref": [
                            "vdoc:selectKey",
                            "#introduction"
                          ]
                        }
                      ]
                    }
                  ]
                },
                "vdoc:content": [
                  "Your answer..."
                ]
              },
              {
                "vdoc:cell": "introduction",
                "@type": "vdoc:Header",
                "vdoc:content": {
                  "vdoc:em": true,
                  "vdoc:content": [
                    "Introduction:"
                  ]
                },
                "vdoc:wide": true,
                "vdoc:tall": true
              },
              {
                "@type": "vdoc:Header",
                "vdoc:content": {
                  "vdoc:em": true,
                  "vdoc:content": [
                    "Aliases:"
                  ]
                },
                "vdoc:wide": true,
                "vdoc:cell": {
                  "vdoc:em": true,
                  "vdoc:content": [
                    {
                      "@type": "vdoc:Reference",
                      "vdoc:content": [
                        {
                          "vdoc:words": {
                            "vdoc:selectField": "subProfiles"
                          }
                        }
                      ],
                      "vdoc:ref": [
                        "vdoc:selectKey",
                        "#section_profiles"
                      ]
                    }
                  ]
                }
              }
            ]
          },
          "vdoc:entries": [
            "technician",
            "valonaut",
            "voyager"
          ]
        }
      ]
    },
    "ontology": {
      "@id": "ontology",
      "dc:title": "Valospace ontology, prefix https://valospace.org/#, preferred label 'valos'",
      "@type": "vdoc:Chapter",
      "vdoc:content": [
        {
          "@id": "section_ontology_abstract"
        },
        {
          "@id": "section_prefixes"
        },
        {
          "@id": "section_types"
        },
        {
          "@id": "section_fields"
        },
        {
          "@id": "section_vocabulary_other"
        },
        {
          "@id": "section_context"
        }
      ]
    },
    "section_ontology_abstract": {
      "@id": "section_ontology_abstract",
      "vdoc:content": [
        "Valospace ontology provides vocabulary and definitions of\n      the primary ValOS resources."
      ]
    },
    "section_prefixes": {
      "@id": "section_prefixes",
      "dc:title": "IRI prefixes",
      "@type": "vdoc:Chapter",
      "vdoc:content": [
        {
          "vdoc:lookup": "prefixes",
          "@type": "vdoc:Table",
          "vdoc:headers": [
            {
              "vdoc:cell": "vdoc:selectKey",
              "@type": "vdoc:Header",
              "vdoc:content": [
                "Prefix"
              ]
            },
            {
              "vdoc:cell": "vdoc:selectValue",
              "@type": "vdoc:Header",
              "vdoc:content": [
                "IRI"
              ]
            }
          ]
        }
      ]
    },
    "section_types": {
      "@id": "section_types",
      "dc:title": "<em>valos:* a valos-raem:Type</em> vocabulary",
      "@type": "vdoc:Chapter",
      "vdoc:content": [
        {
          "vdoc:lookup": "vocabulary",
          "@type": "vdoc:Table",
          "vdoc:headers": {
            "vdoc:entries": [
              {
                "@type": "vdoc:Header",
                "vdoc:content": [
                  "rdfs:label"
                ],
                "vdoc:cell": {
                  "vdoc:resourceId": "vdoc:selectKey",
                  "@type": "vdoc:Reference",
                  "vdoc:content": [
                    {
                      "vdoc:em": true,
                      "vdoc:content": [
                        "vdoc:selectKey"
                      ]
                    }
                  ],
                  "vdoc:ref": [
                    "#",
                    "vdoc:selectKey"
                  ]
                }
              },
              {
                "@type": "vdoc:Header",
                "vdoc:content": [
                  "revdoc:brief"
                ],
                "vdoc:cell": {
                  "vdoc:strong": true,
                  "vdoc:content": [
                    {
                      "vdoc:selectField": "revdoc:brief"
                    }
                  ]
                }
              },
              {
                "@type": "vdoc:Header",
                "vdoc:content": [
                  "rdfs:subClassOf"
                ],
                "vdoc:cell": {
                  "vdoc:words": {
                    "vdoc:selectField": "rdfs:subClassOf"
                  }
                }
              },
              {
                "vdoc:cell": "rdfs:comment",
                "@type": "vdoc:Header",
                "vdoc:content": {
                  "vdoc:em": true,
                  "vdoc:content": [
                    "rdfs:comment"
                  ]
                },
                "vdoc:wide": true
              }
            ]
          },
          "vdoc:entries": [
            "Resource",
            "Bvob",
            "Sourced",
            "Unsourced",
            "Destroyed",
            "Partition",
            "ScriptResource",
            "ScriptDestroyed",
            "ScopeProperty",
            "Scope",
            "Relatable",
            "Relation",
            "Entity",
            "Media"
          ]
        }
      ]
    },
    "section_fields": {
      "@id": "section_fields",
      "dc:title": "<em>valos:* a valos-raem:Field*</em> vocabulary",
      "@type": "vdoc:Chapter",
      "vdoc:content": [
        {
          "vdoc:lookup": "vocabulary",
          "@type": "vdoc:Table",
          "vdoc:headers": {
            "vdoc:entries": [
              {
                "@type": "vdoc:Header",
                "vdoc:content": [
                  "rdfs:label"
                ],
                "vdoc:cell": {
                  "vdoc:resourceId": "vdoc:selectKey",
                  "@type": "vdoc:Reference",
                  "vdoc:content": [
                    {
                      "vdoc:em": true,
                      "vdoc:content": [
                        "vdoc:selectKey"
                      ]
                    }
                  ],
                  "vdoc:ref": [
                    "#",
                    "vdoc:selectKey"
                  ]
                }
              },
              {
                "vdoc:cell": "rdfs:domain",
                "@type": "vdoc:Header",
                "vdoc:content": [
                  "rdfs:domain"
                ]
              },
              {
                "vdoc:cell": "rdfs:range",
                "@type": "vdoc:Header",
                "vdoc:content": [
                  "rdfs:range"
                ]
              },
              {
                "vdoc:cell": "@type",
                "@type": "vdoc:Header",
                "vdoc:content": [
                  "rdf:type"
                ]
              },
              {
                "vdoc:cell": "rdfs:subPropertyOf",
                "@type": "vdoc:Header",
                "vdoc:content": [
                  "rdfs:subPropertyOf"
                ]
              },
              {
                "vdoc:cell": "valos-raem:coupledField",
                "@type": "vdoc:Header",
                "vdoc:content": [
                  "valos-raem:coupledField"
                ]
              },
              {
                "vdoc:cell": "rdfs:comment",
                "@type": "vdoc:Header",
                "vdoc:content": {
                  "vdoc:em": true,
                  "vdoc:content": [
                    "rdfs:comment"
                  ]
                },
                "vdoc:wide": true
              }
            ]
          },
          "vdoc:entries": [
            "id",
            "iri",
            "rawId",
            "typeName",
            "partition",
            "partitionIRI",
            "partitionURI",
            "prototype",
            "derivations",
            "ownFields",
            "inheritancePrototype",
            "inheritors",
            "instancePrototype",
            "instances",
            "ghostPrototype",
            "ghosts",
            "materializedGhosts",
            "unnamedCouplings",
            "ghostHost",
            "ghostOwner",
            "ghostOwnlings",
            "hashAlgorithm",
            "contentHash",
            "contentLength",
            "contentReferrers",
            "owner",
            "name",
            "ownlings",
            "unnamedOwnlings",
            "isFrozen",
            "authorityIRI",
            "partitionAuthorityURI",
            "nameAlias",
            "prototypeAlias",
            "incomingRelations",
            "scope",
            "value",
            "twinspace",
            "subject",
            "predicate",
            "object",
            "properties",
            "relations",
            "source",
            "target",
            "directory",
            "entries",
            "parent",
            "children",
            "container",
            "medias",
            "sourceURL",
            "content",
            "created",
            "modified"
          ]
        }
      ]
    },
    "section_vocabulary_other": {
      "@id": "section_vocabulary_other",
      "dc:title": "<em>valos:</em> other vocabulary",
      "@type": "vdoc:Chapter",
      "vdoc:content": [
        {
          "vdoc:lookup": "vocabulary",
          "@type": "vdoc:Table",
          "vdoc:headers": {
            "vdoc:entries": [
              {
                "@type": "vdoc:Header",
                "vdoc:content": [
                  "rdfs:label"
                ],
                "vdoc:cell": {
                  "vdoc:resourceId": "vdoc:selectKey",
                  "@type": "vdoc:Reference",
                  "vdoc:content": [
                    {
                      "vdoc:em": true,
                      "vdoc:content": [
                        "vdoc:selectKey"
                      ]
                    }
                  ],
                  "vdoc:ref": [
                    "#",
                    "vdoc:selectKey"
                  ]
                }
              },
              {
                "vdoc:cell": "@type",
                "@type": "vdoc:Header",
                "vdoc:content": [
                  "rdf:type"
                ]
              },
              {
                "@type": "vdoc:Header",
                "vdoc:content": [
                  "rdfs:subClassOf"
                ],
                "vdoc:cell": {
                  "vdoc:words": {
                    "vdoc:selectField": "rdfs:subClassOf"
                  }
                }
              },
              {
                "vdoc:cell": "rdfs:comment",
                "@type": "vdoc:Header",
                "vdoc:content": {
                  "vdoc:em": true,
                  "vdoc:content": [
                    "rdfs:comment"
                  ]
                },
                "vdoc:wide": true
              }
            ]
          },
          "vdoc:entries": []
        }
      ]
    },
    "section_context": {
      "@id": "section_context",
      "dc:title": "JSON-LD context term definitions",
      "@type": "vdoc:Chapter",
      "vdoc:content": [
        {
          "vdoc:lookup": "context",
          "@type": "vdoc:Table",
          "vdoc:headers": [
            {
              "vdoc:cell": "vdoc:selectKey",
              "@type": "vdoc:Header",
              "vdoc:content": [
                "Term"
              ]
            },
            {
              "vdoc:cell": "vdoc:selectValue",
              "@type": "vdoc:Header",
              "vdoc:content": [
                "Definition"
              ]
            },
            {
              "vdoc:cell": "@id",
              "@type": "vdoc:Header",
              "vdoc:content": [
                "@id"
              ]
            },
            {
              "vdoc:cell": "@type",
              "@type": "vdoc:Header",
              "vdoc:content": [
                "@type"
              ]
            },
            {
              "vdoc:cell": "@container",
              "@type": "vdoc:Header",
              "vdoc:content": [
                "@container"
              ]
            }
          ]
        }
      ]
    },
    "@type": "revdoc:Document",
    "vdoc:content": [
      {
        "@id": "abstract"
      },
      {
        "@id": "sotd"
      },
      {
        "@id": "introduction"
      },
      {
        "@id": "ontology"
      }
    ]
  }
]